theories/todos.md
@@ -4,5 +4,6 @@ So far we still have a number of works to be done, among which are the following
 
 - [x] Slightly modify the syntax of the expressions; there seems no need to introduce the "lambda calculus" thing. For example, there would be no variables at all... The syntax can thus be simplified.
 - [ ] Implement the noise generator. I am not sure whether if this is directly integrated into the aggregation expressions. It seems to be more natural and easier for us to implement if we just let the type constructor take it as an argument.
+  - [ ] A new type of expression is added as a constructor of `expression`.
 - [ ] Implement the evaluation rule for binary expressions $e_1 \oplus e_2$.
-  - What should be the policy checking logic?
+  - What would be the policy checking logic ??
